WIP call option, verifies with ErrorT autoincs

ContractExamples/FStar/NewCallOptionElaborated.fst
@@ -30,20 +30,19 @@ let tryAddPoint pt utxos =
     7
 
 val tryAddPoints :
-  #l:nat -> V.t outpoint l -> utxos:utxo -> cost (result (V.t pointedOutput l)) M.(20 * l + 20)
+  #l:nat -> V.t outpoint l -> utxos:utxo -> cost (result (V.t pointedOutput l)) M.(17 * l + 17)
 let rec tryAddPoints #l v utxos =
   let open M in
   let open ET in
   Zen.Cost.inc (match v with
-      | V.VNil ->
-        let r : cost (result (V.t pointedOutput l)) (20 * l + 1) = Zen.Cost.inc (ret V.VNil) 1 in r
+      | V.VNil -> let r : cost (result (V.t pointedOutput l)) (17 * l) = ret V.VNil in r
       | V.VCons pt rest ->
         begin match utxos pt with
           | Some oput ->
             do remainder <-- tryAddPoints rest utxos ;
-            inc (ret @ V.VCons (pt, oput) remainder) 1
-          | None -> 20 * l + 1 +! failw "Cannot find output in UTXO set" end)
-    19
+            ret @ V.VCons (pt, oput) remainder
+          | None -> 17 * l +! failw "Cannot find output in UTXO set" end)
+    17
 
 unopteq
 type command =
@@ -52,38 +51,10 @@ type command =
   | Buy : V.t pointedOutput 2 -> outputLock -> command
   | Exercise : V.t pointedOutput 2 -> outputLock -> command
 
-
-
-
-
-
-  (*val makeCommand : inputMsg -> cost (result command) 33
-  let makeCommand imsg =
-    let d : cost (n:nat & inputData n) 3 = Zen.Cost.inc (ret @ imsg.data) 3 in
-    Zen.Cost.inc (do (| n , iData |) <-- d ;
-        do cmd <-- ret @ imsg.cmd ;
-        do utxos <-- ret @ imsg.utxo ;
-        let open M in
-        let open ET in
-        Zen.Cost.inc (match cmd, n with
-            | 0uy, 1 ->
-              begin match iData with
-                | Outpoint pt -> do pointed <-- tryAddPoint pt utxos ; ret @ Initialize pointed
-                | _ -> (inc (failw "Bad Initialization data") 7) <: (cost (result command) 7) end
-            | _ ->
-              let failure : cost (result command) 1 = Zen.Cost.inc (failw "Not implemented") 1 in
-              (Zen.Cost.inc (inc failure 4) 2) <: (cost (result command) 7))
-          14)
-      9*)
-
-
-
-
-
-val makeCommand : inputMsg -> cost (result command) 33
+val makeCommand : inputMsg -> cost (result command) 40
 let makeCommand imsg =
-  let d : cost (n:nat & inputData n) 3 = Zen.Cost.inc (ret @ imsg.data) 3 in
-  Zen.Cost.inc (do (| n , iData |) <-- d ;
+  Zen.Cost.inc (let d : cost (n:nat & inputData n) 0 = ret @ imsg.data in
+      do (| n , iData |) <-- d ;
       do cmd <-- ret @ imsg.cmd ;
       do utxos <-- ret @ imsg.utxo ;
       let open M in
@@ -92,7 +63,68 @@ let makeCommand imsg =
           | 0uy, 1 ->
             begin match iData with
               | Outpoint pt -> do pointed <-- tryAddPoint pt utxos ; ret @ Initialize pointed
-              | _ -> inc (failw "Bad Initialization data") 7  <: (cost (result command) 7) end
-          | _ -> inc (failw "Not implemented") 7  <: (cost (result command) 7))
-        14)
-    9
+              | _ -> autoFailw "Bad Initialization data" end
+          | 0uy, 2 ->
+            begin match iData with
+              | OutpointVector 2 v -> autoFailw "Coll"
+              | _ -> autoFailw "Bad Collateralization data" end
+          | 1uy, 2 ->
+            begin match iData with
+              | Data2 _ _ (OutpointVector 2 v) (OutputLock lk) -> autoFailw "Buy"
+              | _ -> autoFailw "Bad Buy Data" end
+          | 2uy, 2 ->
+            begin match iData with
+              | Data2 _ _ (OutpointVector 2 v) (OutputLock lk) -> autoFailw "Exercise"
+              | _ -> autoFailw "Bad Exercise Data" end
+          | _ -> autoFailw "Not implemented")
+        21)
+    12
+
+
+
+
+
+
+
+
+
+
+
+
+
+
+
+
+
+
+
+
+
+
+
+
+
+
+
+
+
+
+
+
+
+
+
+
+
+
+
+
+
+
+val main : inputMsg -> cost (result transactionSkeleton) 1
+let main iM = Zen.Cost.inc (ET.failw "Not implemented") 1
+
+val cf : inputMsg -> cost nat 1
+let cf _ = Zen.Cost.inc ~!1 1
+val mainFunction : Zen.Types.mainFunction
+let mainFunction = Zen.Types.MainFunc (Zen.Types.CostFunc cf) main
